pipit2/core/Pipit.Exp.Source.fst
@@ -2,6 +2,7 @@ module Pipit.Exp.Source
 
 module PR = Pipit.Exp.Prim
 module PP = Pipit.Exp.Pure
+module PM = Pipit.Base.Prop.Metadata
 module L  = FStar.List.Tot
 
 [@@plugin]
@@ -16,103 +17,128 @@ type nodety = { params: list binder; results: list PR.typ }
 type sigenv = { nodes: list (string & nodety) }
 
 [@@plugin]
-type svar = { svname: nat; svty: PR.typ }
+type svar = { svname: nat; svty: list PR.typ }
 
 [@@plugin]
-type sterm =
-  | SPure    : PP.pterm -> sterm
-  | SVar     : svar -> sterm
-  | SBVar    : nat -> sterm
-  | SFby     : PP.pterm -> sterm -> sterm
-  | SPureApp : PR.prim -> list sterm -> sterm
+type term =
+  | XPure     : PP.pterm -> term
+  | XVar      : svar -> term
+  | XBVar     : nat -> term
+  | XFby      : PP.pterm -> term -> term
+  | XPrim     : PR.prim -> list term -> term
+  | XTuple    : list term -> term
+  | XNode     : string -> list term -> term
+  | XProj     : nat -> term -> term
+  | XMu       : list PR.typ -> term -> term
+  | XLet      : list PR.typ -> term -> term -> term
+  | XContract : PM.contract_status -> term -> term -> term -> term
+  | XCheck    : PM.prop_status -> term -> term
 
-[@@plugin]
-type tterm =
-  | TTuple     : list sterm -> tterm
-  | TStreamApp : string -> list sterm -> tterm
-  | TRec       : list PR.typ -> tterm -> tterm
-  | TLet       : list PR.typ -> tterm -> tterm -> tterm
-
-let rec close_rec_s (k: nat) (x: svar) (e: sterm): Tot sterm (decreases e) =
+let mk_proj (j: nat) (e: term): term =
   match e with
-  | SPure _         -> e
-  | SVar y          -> if y = x then SBVar k else e
-  | SBVar _         -> e
-  | SFby v e'       -> SFby v (close_rec_s k x e')
-  | SPureApp h args -> SPureApp h (close_args_s k x args)
-and close_args_s (k: nat) (x: svar) (args: list sterm): Tot (list sterm) (decreases args) =
+  | XTuple es -> if j < L.length es then L.index es j else XProj j e
+  | _         -> XProj j e
+
+let rec close_rec (k: nat) (x: svar) (e: term): Tot term (decreases e) =
+  match e with
+  | XPure _           -> e
+  | XVar y            -> if y = x then XBVar k else e
+  | XBVar _           -> e
+  | XFby v e'         -> XFby v (close_rec k x e')
+  | XPrim p args      -> XPrim p (close_args k x args)
+  | XTuple es         -> XTuple (close_args k x es)
+  | XNode nm args     -> XNode nm (close_args k x args)
+  | XProj j e'        -> XProj j (close_rec k x e')
+  | XMu tys body      -> XMu tys (close_rec (k + 1) x body)
+  | XLet tys rhs bod  -> XLet tys (close_rec k x rhs) (close_rec (k + 1) x bod)
+  | XContract s r g i -> XContract s (close_rec k x r) (close_rec (k + 1) x g) (close_rec k x i)
+  | XCheck s e'       -> XCheck s (close_rec k x e')
+and close_args (k: nat) (x: svar) (args: list term): Tot (list term) (decreases args) =
   match args with
   | []      -> []
-  | a :: tl -> close_rec_s k x a :: close_args_s k x tl
+  | a :: tl -> close_rec k x a :: close_args k x tl
 
-let rec close_rec_t (k: nat) (x: svar) (t: tterm): Tot tterm (decreases t) =
-  match t with
-  | TTuple es          -> TTuple (close_args_s k x es)
-  | TStreamApp nm args -> TStreamApp nm (close_args_s k x args)
-  | TRec tys body      -> TRec tys (close_rec_t (k + L.length tys) x body)
-  | TLet tys rhs bod   -> TLet tys (close_rec_t k x rhs) (close_rec_t (k + L.length tys) x bod)
-
-let rec open_rec_s (k: nat) (u: sterm) (e: sterm): Tot sterm (decreases e) =
+let rec open_rec (k: nat) (u: term) (e: term): Tot term (decreases e) =
   match e with
-  | SPure _         -> e
-  | SVar _          -> e
-  | SBVar i         -> if i = k then u else e
-  | SFby v e'       -> SFby v (open_rec_s k u e')
-  | SPureApp h args -> SPureApp h (open_args_s k u args)
-and open_args_s (k: nat) (u: sterm) (args: list sterm): Tot (list sterm) (decreases args) =
+  | XPure _           -> e
+  | XVar _            -> e
+  | XBVar i           -> if i = k then u else e
+  | XFby v e'         -> XFby v (open_rec k u e')
+  | XPrim p args      -> XPrim p (open_args k u args)
+  | XTuple es         -> XTuple (open_args k u es)
+  | XNode nm args     -> XNode nm (open_args k u args)
+  | XProj j e'        -> mk_proj j (open_rec k u e')
+  | XMu tys body      -> XMu tys (open_rec (k + 1) u body)
+  | XLet tys rhs bod  -> XLet tys (open_rec k u rhs) (open_rec (k + 1) u bod)
+  | XContract s r g i -> XContract s (open_rec k u r) (open_rec (k + 1) u g) (open_rec k u i)
+  | XCheck s e'       -> XCheck s (open_rec k u e')
+and open_args (k: nat) (u: term) (args: list term): Tot (list term) (decreases args) =
   match args with
   | []      -> []
-  | a :: tl -> open_rec_s k u a :: open_args_s k u tl
+  | a :: tl -> open_rec k u a :: open_args k u tl
 
-let rec open_rec_t (k: nat) (u: sterm) (t: tterm): Tot tterm (decreases t) =
-  match t with
-  | TTuple es          -> TTuple (open_args_s k u es)
-  | TStreamApp nm args -> TStreamApp nm (open_args_s k u args)
-  | TRec tys body      -> TRec tys (open_rec_t (k + L.length tys) u body)
-  | TLet tys rhs bod   -> TLet tys (open_rec_t k u rhs) (open_rec_t (k + L.length tys) u bod)
+let close (x: svar) (e: term): term = close_rec 0 x e
 
-let close (x: svar) (e: sterm): sterm = close_rec_s 0 x e
+let open_var (x: svar) (e: term): term = open_rec 0 (XVar x) e
 
-let open_var (x: svar) (e: sterm): sterm = open_rec_s 0 (SVar x) e
+let subst_tuple (def: term) (body: term): term = open_rec 0 def body
 
-let rec infer_s (env: sigenv) (ctx: list PR.typ) (e: sterm): Tot (option PR.typ) (decreases e) =
+let rec infer (env: sigenv) (ctx: list (list PR.typ)) (e: term)
+: Tot (option (list PR.typ)) (decreases e) =
   match e with
-  | SPure v         -> PP.infer_p v
-  | SVar x          -> Some x.svty
-  | SBVar i         -> if i < L.length ctx then Some (L.index ctx i) else None
-  | SFby v e'       -> (match PP.infer_p v with
-                       | Some a -> if infer_s env ctx e' = Some a then Some a else None
-                       | None   -> None)
-  | SPureApp p args -> (match infer_sargs env ctx args with
-                       | Some tys -> PR.prim_ty p tys
-                       | None     -> None)
-and infer_sargs (env: sigenv) (ctx: list PR.typ) (args: list sterm)
+  | XPure p        -> (match PP.pterm_ty PP.ty_empty p with
+                      | Some a -> Some [a]
+                      | None   -> None)
+  | XVar x         -> Some x.svty
+  | XBVar i        -> if i < L.length ctx then Some (L.index ctx i) else None
+  | XFby v e'      -> (match PP.pterm_ty PP.ty_empty v with
+                      | Some a -> if infer env ctx e' = Some [a] then Some [a] else None
+                      | None   -> None)
+  | XPrim p args   -> (match infer_scalars env ctx args with
+                      | Some tys -> (match PR.prim_ty p tys with
+                                    | Some r -> Some [r]
+                                    | None   -> None)
+                      | None     -> None)
+  | XTuple es      -> infer_widths env ctx es
+  | XNode nm args  -> (match L.assoc nm env.nodes with
+                      | Some nt -> if check_node_args env ctx args nt.params
+                                  then Some nt.results else None
+                      | None    -> None)
+  | XProj j e'     -> (match infer env ctx e' with
+                      | Some tys -> if j < L.length tys then Some [L.index tys j] else None
+                      | None     -> None)
+  | XMu tys body   -> if infer env (tys :: ctx) body = Some tys then Some tys else None
+  | XLet tys d b   -> if infer env ctx d = Some tys
+                     then infer env (tys :: ctx) b else None
+  | XContract s r g i ->
+    (match infer env ctx i with
+     | Some tys -> if infer env ctx r = Some [PR.TBool] && infer env (tys :: ctx) g = Some [PR.TBool]
+                  then Some tys else None
+     | None     -> None)
+  | XCheck s e'    -> if infer env ctx e' = Some [PR.TBool] then Some [] else None
+and infer_scalars (env: sigenv) (ctx: list (list PR.typ)) (args: list term)
 : Tot (option (list PR.typ)) (decreases args) =
   match args with
   | []      -> Some []
-  | a :: tl -> (match infer_s env ctx a, infer_sargs env ctx tl with
-               | Some t, Some ts -> Some (t :: ts)
+  | a :: tl -> (match infer env ctx a, infer_scalars env ctx tl with
+               | Some [t], Some ts -> Some (t :: ts)
+               | _, _              -> None)
+and infer_widths (env: sigenv) (ctx: list (list PR.typ)) (es: list term)
+: Tot (option (list PR.typ)) (decreases es) =
+  match es with
+  | []      -> Some []
+  | e :: tl -> (match infer env ctx e, infer_widths env ctx tl with
+               | Some w, Some ws -> Some (L.append w ws)
                | _, _            -> None)
-and check_node_args (env: sigenv) (ctx: list PR.typ) (args: list sterm) (params: list binder)
+and check_node_args (env: sigenv) (ctx: list (list PR.typ)) (args: list term) (params: list binder)
 : Tot bool (decreases args) =
   match args, params with
   | [], []                     -> true
-  | a :: atl, BStream t :: ptl -> infer_s env ctx a = Some t && check_node_args env ctx atl ptl
+  | a :: atl, BStream t :: ptl -> infer env ctx a = Some [t] && check_node_args env ctx atl ptl
   | a :: atl, BConst t :: ptl  ->
-    (match a with SPure v -> PP.infer_p v = Some t | _ -> false) && check_node_args env ctx atl ptl
+    (match a with XPure v -> PP.pterm_ty PP.ty_empty v = Some t | _ -> false)
+    && check_node_args env ctx atl ptl
   | _, _                       -> false
 
-let rec infer_t (env: sigenv) (ctx: list PR.typ) (t: tterm): Tot (option (list PR.typ)) (decreases t) =
-  match t with
-  | TTuple es          -> infer_sargs env ctx es
-  | TStreamApp nm args -> (match L.assoc nm env.nodes with
-                          | Some nt -> if check_node_args env ctx args nt.params
-                                      then Some nt.results else None
-                          | None    -> None)
-  | TRec tys body      -> if infer_t env (L.append tys ctx) body = Some tys
-                         then Some tys else None
-  | TLet tys rhs bod   -> if infer_t env ctx rhs = Some tys
-                         then infer_t env (L.append tys ctx) bod else None
-
-let well_typed (env: sigenv) (ctx: list PR.typ) (e: sterm) (a: PR.typ): prop =
-  infer_s env ctx e == Some a
+let well_typed (env: sigenv) (ctx: list (list PR.typ)) (e: term) (w: list PR.typ): prop =
+  infer env ctx e == Some w
