pipit2/core/Pipit.Source.Stream.fst
@@ -5,59 +5,56 @@ module PP  = Pipit.Exp.Pure
 module PES = Pipit.Exp.Source
 module L   = FStar.List.Tot
 
-type stream (ts: list PR.typ) = nat -> PES.tterm & nat
+type stream (ts: list PR.typ) = nat -> PES.term & nat
 
-let fresh (a: PR.typ) (n: nat): PES.svar & nat =
+let fresh (a: list PR.typ) (n: nat): PES.svar & nat =
   ({ PES.svname = n; svty = a }, n + 1)
 
-let rec fresh_vars (ts: list PR.typ) (n: nat): list PES.svar & nat =
-  match ts with
-  | []      -> ([], n)
-  | a :: tl -> let (x, n)  = fresh a n in
-               let (xs, n) = fresh_vars tl n in
-               (x :: xs, n)
+let rec proj_refs (g: PES.svar) (j: nat) (tys: list PR.typ)
+: Tot (list PES.term) (decreases tys) =
+  match tys with
+  | []      -> []
+  | _ :: tl -> PES.XProj j (PES.XVar g) :: proj_refs g (j + 1) tl
 
-let rec close_vars (k: nat) (xs: list PES.svar) (body: PES.tterm): Tot PES.tterm (decreases xs) =
-  match xs with
-  | []      -> body
-  | x :: tl -> PES.close_rec_t k x (close_vars (k + 1) tl body)
+let refs (g: PES.svar): list PES.term =
+  match g.svty with
+  | [_] -> [PES.XVar g]
+  | tys -> proj_refs g 0 tys
 
-let atomize (a: PR.typ) (t: PES.tterm) (n: nat)
-: PES.sterm & (PES.tterm -> PES.tterm) & nat =
+let atomize (a: PR.typ) (t: PES.term) (n: nat)
+: PES.term & (PES.term -> PES.term) & nat =
   match t with
-  | PES.TTuple [e] -> (e, (fun body -> body), n)
+  | PES.XTuple [e] -> (e, (fun body -> body), n)
   | _ ->
-    let (x, n) = fresh a n in
-    (PES.SVar x, (fun body -> PES.TLet [a] t (PES.close_rec_t 0 x body)), n)
+    let (g, n) = fresh [a] n in
+    (PES.XVar g, (fun body -> PES.XLet [a] t (PES.close g body)), n)
 
-let components (ts: list PR.typ) (t: PES.tterm) (n: nat)
-: list PES.sterm & (PES.tterm -> PES.tterm) & nat =
+let components (ts: list PR.typ) (t: PES.term) (n: nat)
+: list PES.term & (PES.term -> PES.term) & nat =
   match t with
-  | PES.TTuple es -> (es, (fun body -> body), n)
+  | PES.XTuple es -> (es, (fun body -> body), n)
   | _ ->
-    let (xs, n) = fresh_vars ts n in
-    (L.map (fun (x: PES.svar) -> PES.SVar x) xs,
-     (fun body -> PES.TLet ts t (close_vars 0 xs body)),
-     n)
+    let (g, n) = fresh ts n in
+    (refs g, (fun body -> PES.XLet ts t (PES.close g body)), n)
 
 let fvar (#a: PR.typ) (x: PES.svar): stream [a] =
-  fun n -> (PES.TTuple [PES.SVar x], n)
+  fun n -> (PES.XTuple [PES.XVar x], n)
 
 let const (#a: PR.typ) (v: PP.pterm): stream [a] =
-  fun n -> (PES.TTuple [PES.SPure v], n)
+  fun n -> (PES.XTuple [PES.XPure v], n)
 
 let fby (#a: PR.typ) (v: PP.pterm) (s: stream [a]): stream [a] =
   fun n ->
     let (t, n)    = s n in
     let (e, w, n) = atomize a t n in
-    (w (PES.TTuple [PES.SFby v e]), n)
+    (w (PES.XTuple [PES.XFby v e]), n)
 
 let liftP (#args: list PR.typ) (#result: PR.typ)
     (p: PR.prim) (s: stream args): stream [result] =
   fun n ->
     let (t, n)     = s n in
     let (es, w, n) = components args t n in
-    (w (PES.TTuple [PES.SPureApp p es]), n)
+    (w (PES.XTuple [PES.XPrim p es]), n)
 
 let zips (#xs #ys: list PR.typ) (x: stream xs) (y: stream ys): stream (L.append xs ys) =
   fun n ->
@@ -65,18 +62,18 @@ let zips (#xs #ys: list PR.typ) (x: stream xs) (y: stream ys): stream (L.append 
     let (exs, wx, n) = components xs tx n in
     let (ty, n)      = y n in
     let (eys, wy, n) = components ys ty n in
-    (wx (wy (PES.TTuple (L.append exs eys))), n)
+    (wx (wy (PES.XTuple (L.append exs eys))), n)
 
 let unzips (#xs #ys: list PR.typ) (s: stream (L.append xs ys)): stream xs & stream ys =
   let k = L.length xs in
   ( (fun n ->
       let (t, n)     = s n in
       let (es, w, n) = components (L.append xs ys) t n in
-      (w (PES.TTuple (fst (L.splitAt k es))), n))
+      (w (PES.XTuple (fst (L.splitAt k es))), n))
   , (fun n ->
       let (t, n)     = s n in
       let (es, w, n) = components (L.append xs ys) t n in
-      (w (PES.TTuple (snd (L.splitAt k es))), n)) )
+      (w (PES.XTuple (snd (L.splitAt k es))), n)) )
 
 let zip2 (#a: PR.typ) (#b: list PR.typ)
     (x: stream [a]) (y: stream b): stream (a :: b) =
@@ -100,17 +97,17 @@ let let' (#a #b: list PR.typ)
     (e: stream a) (f: stream a -> stream b): stream b =
   fun n ->
     let (ev, n)    = e n in
-    let (xs, n)    = fresh_vars a n in
-    let sref: stream a = (fun m -> (PES.TTuple (L.map (fun (x: PES.svar) -> PES.SVar x) xs), m)) in
+    let (g, n)     = fresh a n in
+    let sref: stream a = (fun m -> (PES.XTuple (refs g), m)) in
     let (bodyv, n) = f sref n in
-    (PES.TLet a ev (close_vars 0 xs bodyv), n)
+    (PES.XLet a ev (PES.close g bodyv), n)
 
 let mu (#a: list PR.typ) (f: stream a -> stream a): stream a =
   fun n ->
-    let (xs, n)    = fresh_vars a n in
-    let sref: stream a = (fun m -> (PES.TTuple (L.map (fun (x: PES.svar) -> PES.SVar x) xs), m)) in
+    let (g, n)     = fresh a n in
+    let sref: stream a = (fun m -> (PES.XTuple (refs g), m)) in
     let (bodyv, n) = f sref n in
-    (PES.TRec a (close_vars 0 xs bodyv), n)
+    (PES.XMu a (PES.close g bodyv), n)
 
 let letrec (#a #b: list PR.typ)
     (f: stream a -> stream a) (cont: stream a -> stream b): stream b =
@@ -121,7 +118,7 @@ let node (#args #results: list PR.typ)
   fun n ->
     let (t, n)     = s n in
     let (es, w, n) = components args t n in
-    (w (PES.TStreamApp head es), n)
+    (w (PES.XNode head es), n)
 
-let exp_of_stream (#a: list PR.typ) (s: stream a): PES.tterm =
+let exp_of_stream (#a: list PR.typ) (s: stream a): PES.term =
   fst (s 0)
