pipit2/plugin-test/Pipit.Test.Node.fst
@@ -18,26 +18,26 @@ let src: S.stream [EB.bool_ty] =
   in
   S.liftP PR.PAnd (S.zip2 o1 o2)
 
-let term: PES.tterm = S.exp_of_stream src
+let term: PES.term = S.exp_of_stream src
 
-let capp: PES.tterm =
-  PES.TStreamApp "ctrl" [PES.SPure btrue; PES.SPure bfalse]
+let capp: PES.term =
+  PES.XNode "ctrl" [PES.XPure btrue; PES.XPure bfalse]
 
-let o_proj (i: nat) : PES.tterm =
-  PES.TLet [EB.bool_ty; EB.bool_ty] capp (PES.TTuple [PES.SBVar i])
+let o_proj (i: nat) : PES.term =
+  PES.XLet [EB.bool_ty; EB.bool_ty] capp (PES.XTuple [PES.XProj i (PES.XBVar 0)])
 
-let expected: PES.tterm =
-  PES.TLet [EB.bool_ty; EB.bool_ty]
-    (PES.TLet [EB.bool_ty] (o_proj 0)
-      (PES.TLet [EB.bool_ty] (o_proj 1)
-        (PES.TTuple [PES.SBVar 1; PES.SBVar 0])))
-    (PES.TTuple [PES.SPureApp PR.PAnd [PES.SBVar 0; PES.SBVar 1]])
+let expected: PES.term =
+  PES.XLet [EB.bool_ty; EB.bool_ty]
+    (PES.XLet [EB.bool_ty] (o_proj 0)
+      (PES.XLet [EB.bool_ty] (o_proj 1)
+        (PES.XTuple [PES.XBVar 1; PES.XBVar 0])))
+    (PES.XTuple [PES.XPrim PR.PAnd [PES.XProj 0 (PES.XBVar 0); PES.XProj 1 (PES.XBVar 0)]])
 
 let node_lowers_ok (): Lemma (term == expected) =
   assert_norm (term == expected)
 
-let node_typechecks (): Lemma (PES.infer_t EB.benv [] capp == Some [EB.bool_ty; EB.bool_ty]) =
-  assert_norm (PES.infer_t EB.benv [] capp == Some [EB.bool_ty; EB.bool_ty])
+let node_typechecks (): Lemma (PES.infer EB.benv [] capp == Some [EB.bool_ty; EB.bool_ty]) =
+  assert_norm (PES.infer EB.benv [] capp == Some [EB.bool_ty; EB.bool_ty])
 
 let anf_expected: A.cont =
   A.CLetNode "ctrl" [A.APure btrue; A.APure bfalse] [PR.TBool; PR.TBool]
