pipit2/plugin-test/Pipit.Test.Rec.fst
@@ -10,35 +10,35 @@ let i0 : PP.pterm = PP.PValue (PR.VInt 0)
 let i1 : PP.pterm = PP.PValue (PR.VInt 1)
 
 (* `a = 0 fby b  and  b = 1 fby a` *)
-let rec_ab : PES.tterm =
-  PES.TRec [PR.TInt; PR.TInt]
-    (PES.TTuple
-      [ PES.SFby i0 (PES.SBVar 1)
-      ; PES.SFby i1 (PES.SBVar 0) ])
+let rec_ab : PES.term =
+  PES.XMu [PR.TInt; PR.TInt]
+    (PES.XTuple
+      [ PES.XFby i0 (PES.XProj 1 (PES.XBVar 0))
+      ; PES.XFby i1 (PES.XProj 0 (PES.XBVar 0)) ])
 
-let _ = assert_norm (PES.infer_t env [] rec_ab == Some [PR.TInt; PR.TInt])
+let _ = assert_norm (PES.infer env [] rec_ab == Some [PR.TInt; PR.TInt])
 
-let proj (i: nat) : PES.tterm =
-  PES.TLet [PR.TInt; PR.TInt] rec_ab (PES.TTuple [PES.SBVar i])
+let proj (i: nat) : PES.term =
+  PES.XLet [PR.TInt; PR.TInt] rec_ab (PES.XTuple [PES.XProj i (PES.XBVar 0)])
 
-let _ = assert_norm (PES.infer_t env [] (proj 0) == Some [PR.TInt])
-let _ = assert_norm (PES.infer_t env [] (proj 1) == Some [PR.TInt])
+let _ = assert_norm (PES.infer env [] (proj 0) == Some [PR.TInt])
+let _ = assert_norm (PES.infer env [] (proj 1) == Some [PR.TInt])
 
-let _ = assert_norm (PES.infer_t env [] (proj 2) == None)
+let _ = assert_norm (PES.infer env [] (proj 2) == None)
 
-let x : PES.svar = { PES.svname = 0; svty = PR.TInt }
+let x : PES.svar = { PES.svname = 0; svty = [PR.TInt] }
 
-let grp_open : PES.tterm =
-  PES.TRec [PR.TInt; PR.TInt]
-    (PES.TTuple
-      [ PES.SFby i0 (PES.SVar x)
-      ; PES.SFby i1 (PES.SBVar 0) ])
+let grp_open : PES.term =
+  PES.XMu [PR.TInt; PR.TInt]
+    (PES.XTuple
+      [ PES.XFby i0 (PES.XVar x)
+      ; PES.XFby i1 (PES.XProj 0 (PES.XBVar 0)) ])
 
-let grp_closed : PES.tterm =
-  PES.TRec [PR.TInt; PR.TInt]
-    (PES.TTuple
-      [ PES.SFby i0 (PES.SBVar 2)
-      ; PES.SFby i1 (PES.SBVar 0) ])
+let grp_closed : PES.term =
+  PES.XMu [PR.TInt; PR.TInt]
+    (PES.XTuple
+      [ PES.XFby i0 (PES.XBVar 1)
+      ; PES.XFby i1 (PES.XProj 0 (PES.XBVar 0)) ])
 
-let _ = assert_norm (PES.close_rec_t 0 x grp_open == grp_closed)
-let _ = assert_norm (PES.open_rec_t 0 (PES.SVar x) grp_closed == grp_open)
+let _ = assert_norm (PES.close_rec 0 x grp_open == grp_closed)
+let _ = assert_norm (PES.open_rec 0 (PES.XVar x) grp_closed == grp_open)
