pipit2/base/Pipit.Base.Context.Named.fst
@@ -1,0 +1,15 @@
+module Pipit.Base.Context.Named
+
+module L = FStar.List.Tot
+
+unfold
+type context (a: Type) = list (string & a)
+
+inline_for_extraction
+let empty (#a: Type): context a = []
+
+inline_for_extraction
+let lookup (#a: Type) (c: context a) (x: string): option a = L.assoc x c
+
+inline_for_extraction
+let update (#a: Type) (c: context a) (x: string) (v: a): context a = (x, v) :: c
