pipit2/base/Pipit.Base.Context.fst
@@ -1,0 +1,26 @@
+module Pipit.Base.Context
+
+module L = FStar.List.Tot
+
+type context (a: Type) = list a
+
+let index = nat
+
+let has_index (c: context 'a) (i: index): bool = i < L.length c
+
+let get_index (c: context 'a) (i: index { has_index c i }): 'a = L.index c i
+
+let opt_index (c: context 'a) (i: index): option 'a =
+  if has_index c i then Some (get_index c i) else None
+
+let empty (#a: Type): context a = []
+
+let close1 (c: context 'a) (t: 'a): context 'a = t :: c
+
+let open1 (c: context 'a { has_index c 0 }): context 'a = L.tl c
+
+let index_lift (i limit: index): index = if i >= limit then i + 1 else i
+
+let index_drop (i limit: index): index = if i > limit then i - 1 else i
+
+let index_lifts (i limit: index) (n: nat): index = if i >= limit then i + n else i
