pipit2/base/Pipit.Base.Prop.Metadata.fst
@@ -1,0 +1,15 @@
+module Pipit.Base.Prop.Metadata
+
+[@@plugin]
+type prop_status = | PSValid | PSUnknown
+
+type contract_status = prop_status
+
+let contract_status_unknown: contract_status = PSUnknown
+
+type check_mode = prop_status
+
+let prop_status_contains (s: check_mode) (p: prop_status): bool = s = p
+
+let check_mode_valid:   check_mode = PSValid
+let check_mode_unknown: check_mode = PSUnknown
