pipit2/core/Pipit.Transform.Rewrite.fst
@@ -2,25 +2,25 @@ module Pipit.Transform.Rewrite
 
 module PES = Pipit.Exp.Source
 
-let rec rewrite (step: PES.sterm -> PES.sterm) (e: PES.sterm): Tot PES.sterm (decreases e) =
-  let e': PES.sterm =
+let rec rewrite (step: PES.term -> PES.term) (e: PES.term): Tot PES.term (decreases e) =
+  let e': PES.term =
     match e with
-    | PES.SPure _         -> e
-    | PES.SVar _          -> e
-    | PES.SBVar _         -> e
-    | PES.SFby v b        -> PES.SFby v (rewrite step b)
-    | PES.SPureApp h args -> PES.SPureApp h (rewrite_args step args)
+    | PES.XPure _           -> e
+    | PES.XVar _            -> e
+    | PES.XBVar _           -> e
+    | PES.XFby v b          -> PES.XFby v (rewrite step b)
+    | PES.XPrim h args      -> PES.XPrim h (rewrite_args step args)
+    | PES.XTuple es         -> PES.XTuple (rewrite_args step es)
+    | PES.XNode nm args     -> PES.XNode nm (rewrite_args step args)
+    | PES.XProj j b         -> PES.XProj j (rewrite step b)
+    | PES.XMu tys body      -> PES.XMu tys (rewrite step body)
+    | PES.XLet tys rhs bod  -> PES.XLet tys (rewrite step rhs) (rewrite step bod)
+    | PES.XContract s r g i -> PES.XContract s (rewrite step r) (rewrite step g) (rewrite step i)
+    | PES.XCheck s b        -> PES.XCheck s (rewrite step b)
   in
   step e'
-and rewrite_args (step: PES.sterm -> PES.sterm) (args: list PES.sterm)
-: Tot (list PES.sterm) (decreases args) =
+and rewrite_args (step: PES.term -> PES.term) (args: list PES.term)
+: Tot (list PES.term) (decreases args) =
   match args with
   | []      -> []
   | a :: tl -> rewrite step a :: rewrite_args step tl
-
-let rec rewrite_t (step: PES.sterm -> PES.sterm) (t: PES.tterm): Tot PES.tterm (decreases t) =
-  match t with
-  | PES.TTuple es          -> PES.TTuple (rewrite_args step es)
-  | PES.TStreamApp nm args -> PES.TStreamApp nm (rewrite_args step args)
-  | PES.TRec tys body      -> PES.TRec tys (rewrite_t step body)
-  | PES.TLet tys rhs bod   -> PES.TLet tys (rewrite_t step rhs) (rewrite_t step bod)
